add: an example simple graph

LeanExcerciseGraphTheory/Graph.lean
@@ -1,3 +1,6 @@
+import Mathlib.Data.Finset.Basic
+import Mathlib.Data.Finset.Defs
+
 universe u
 class Graph' (V : Type u) where
   adj : V → V → Prop
@@ -5,3 +8,41 @@ class Graph' (V : Type u) where
 class SimpleGraph (V : Type u) extends Graph' V where
   symm : ∀ a : V, ∀ b : V, adj a b = adj b a
   noLoop : ∀ a : V, ¬ adj a a
+
+def example_vertecies : Finset Nat := {1, 2, 3, 4}
+def example_adj : {x // x ∈ example_vertecies} → {x // x ∈ example_vertecies} → Prop
+  | ⟨1, _⟩, ⟨2, _⟩ => True
+  | ⟨2, _⟩, ⟨1, _⟩ => True
+  | _, _ => False
+
+lemma example_adj_symm :
+    ∀ (a b : {x // x ∈ example_vertecies}), example_adj a b = example_adj b a := by
+  intro a b
+  -- a と b を分解
+  obtain ⟨av, ah⟩ := a
+  obtain ⟨bv, bh⟩ := b
+  simp only [example_adj]
+  -- 具体的な値での証明
+  simp only [example_vertecies] at ah bh
+  rw [Finset.mem_insert, Finset.mem_insert, Finset.mem_insert, Finset.mem_singleton] at ah bh
+  -- すべてのケースを網羅
+  rcases ah with (rfl | rfl | rfl | rfl) <;>
+  rcases bh with (rfl | rfl | rfl | rfl) <;>
+  rfl
+
+lemma example_no_loop :
+    ∀ a : {x // x ∈ example_vertecies}, ¬ example_adj a a := by
+  intro a
+  obtain ⟨av, ah⟩ := a
+  simp only [example_adj]
+  -- 具体的な値での証明
+  simp only [example_vertecies] at ah
+  rw [Finset.mem_insert, Finset.mem_insert, Finset.mem_insert, Finset.mem_singleton] at ah
+  -- 各ケースを確認
+  rcases ah with (rfl | rfl | rfl | rfl) <;> decide
+
+def example_simple_graph : SimpleGraph (example_vertecies) :=
+  { adj := example_adj,
+    symm := example_adj_symm,
+    noLoop := example_no_loop
+  }
